analysis/markov/Linleios/Evolve.lean
@@ -11,28 +11,36 @@ open Lean.ToJson (toJson)
 open Std (HashMap)
 
 
-def certify {env : Environment} (state : State) : Outcomes :=
+def forge {env : Environment} (state : State) : Outcomes :=
   let state' :=
     {
       state with
-      rbCount := state.rbCount + 1
-      canCertify := true
+      clock := state.clock + 1
     }
+  let p := 1 - env.fAdversary
+  [
+    ({state' with rbCount := state.rbCount + 1}, p)
+  , (state', 1 - p)
+  ]
+
+def certify {env : Environment} (state : State) : Outcomes :=
+  let p := env.pSpacingOkay * (1 - env.fAdversary)
   if state.canCertify
     then [
-           ⟨{state' with ebCount := state.ebCount + 1}, env.pSpacingOkay⟩
-         , ⟨state', 1 - env.pSpacingOkay⟩
+           ⟨{state with ebCount := state.ebCount + 1}, p⟩
+         , ⟨state, 1 - p⟩
          ]
-    else [(state', 1)]
+    else [(state, 1)]
 
 def vote {env : Environment} (state : State) : Outcomes :=
+  let p := env.pQuorum * (1 - env.fAdversary)
   [
-    (state, env.pQuorum)
-  , ({state with canCertify := false}, 1 - env.pQuorum)
+    ({state with canCertify := true}, p)
+  , ({state with canCertify := false}, 1 - p)
   ]
 
 def step {env : Environment} : List (State → Outcomes) :=
-  [@certify env, @vote env]
+  [@forge env, @certify env, @vote env]
 
 
 def prune (ε : Float) : Probabilities → Probabilities :=
@@ -75,10 +83,10 @@ def ebDistributionJson : Probabilities → Json :=
   Json.mkObj ∘ List.map (fun ⟨k, v⟩ => ⟨toString k, toJson v⟩) ∘ HashMap.toList ∘ ebDistribution
 
 def ebEfficiency (states : Probabilities) : Float :=
-  let rbCount := states.keys.head!.rbCount
+  let clock := states.keys.head!.clock
   let ebCount :=
     HashMap.fold
       (fun acc state p =>acc + state.ebCount.toFloat * p)
       0
       states
-  ebCount / (rbCount.toFloat - 1)
+  ebCount / (clock.toFloat - 1)
